StructuredEncryption/src/AwsCryptographyStructuredEncryptionOperations.dfy
@@ -1,48 +1,49 @@
 // Copyright Amazon.com Inc. or its affiliates. All Rights Reserved.
 // SPDX-License-Identifier: Apache-2.0
 include "../Model/AwsCryptographyStructuredEncryptionTypes.dfy"
-include "../../private-aws-encryption-sdk-dafny-staging/AwsCryptographicMaterialProviders/test/TestUtils.dfy"
+
 include "Header.dfy"
+include "Paths.dfy"
+include "Crypt.dfy"
+include "Util.dfy"
 
 module AwsCryptographyStructuredEncryptionOperations refines AbstractAwsCryptographyStructuredEncryptionOperations {
+  import opened StructuredEncryptionUtil
+
   import Base64
   import CMP = AwsCryptographyMaterialProvidersTypes
+  import CSE = AwsCryptographyStructuredEncryptionTypes
+  import Prim = AwsCryptographyPrimitivesTypes
   import Random
   import Aws.Cryptography.Primitives
-  import Header
+  import Header = StructuredEncryptionHeader
   import MaterialProviders
-  import TestUtils
+  import Materials
+  import Crypt = StructuredEncryptionCrypt
+  import Paths = StructuredEncryptionPaths
+  import Sets
+  import Seq
+  import Digest
+  import Defaults
+  import HKDF
+  import AlgorithmSuites
 
   datatype Config = Config(
-    primatives : Primitives.AtomicPrimitivesClient
+    primitives : Primitives.AtomicPrimitivesClient
   )
 
   type InternalConfig = Config
 
-  // UTF-8 encoded "THIS_IS_NOT_ENCRYPTED"
-  // TODO this is temporary, only used for our "fake" encryption
-  // in order to make it clear that the value is not actually being encrypted yet.
-  const THIS_IS_NOT_ENCRYPTED: UTF8.ValidUTF8Bytes :=
-    var s := [0x54, 0x48, 0x49, 0x53, 0x5f, 0x49, 0x53, 0x5f, 0x4e, 0x4f, 0x54, 0x5f, 0x45, 0x4e, 0x43, 0x52, 0x59, 0x50, 0x54, 0x45, 0x44];
-    assert UTF8.ValidUTF8Range(s, 0, 21);
-    s
-
   const DBE_COMMITMENT_POLICY := CMP.CommitmentPolicy.DBE(CMP.DBECommitmentPolicy.REQUIRE_ENCRYPT_REQUIRE_DECRYPT)
 
-  // TODO: This is temporary in order to support "fake" encryption with DDB,
-  // which is a placeholder to demonstrate the crypto schema is piping to this
-  // layer as expected when testing end to end with the DDB Encryption interceptor.
-  const DDB_STRING_TYPE_ID : seq<uint8> := [0x00, 0x01];
-  const BYTES_TYPE_ID : seq<uint8> := [0xFF, 0xFF];
-
   predicate ValidInternalConfig?(config: InternalConfig)
-  {config.primatives.ValidState()}
+  {config.primitives.ValidState()}
 
   function ModifiesInternalConfig(config: InternalConfig) : set<object>
-  {config.primatives.Modifies}
+  {config.primitives.Modifies}
 
   predicate EncryptStructureEnsuresPublicly(
-    input: EncryptStructureInput, 
+    input: EncryptStructureInput,
     output: Result<EncryptStructureOutput, Error>) {
       // Input and output types must be the same, and this constraint is useful to Dafny users
     && (output.Success? && input.plaintextStructure.content.DataMap? ==> output.value.encryptedStructure.content.DataMap?)
@@ -50,184 +51,475 @@ module AwsCryptographyStructuredEncryptionOperations refines AbstractAwsCryptogr
     && (output.Success? && input.plaintextStructure.content.Terminal? ==> output.value.encryptedStructure.content.Terminal?)
   }
 
-  method EncryptStructure(config: InternalConfig, input: EncryptStructureInput)
-    returns (output: Result<EncryptStructureOutput, Error>)
+  // given a list of fields, return only those that should be encrypted, according to the legend
+  function method {:tailrecursion} {:opaque} FilterEncrypted(fields : seq<CanonicalPath>, legend : Header.Legend)
+    : (ret : seq<CanonicalPath>)
+    requires |fields| == |legend|
+    ensures forall k <- ret :: k in fields
   {
-    var algorithmSuiteId := if input.algorithmSuiteId.Some? then
-      Some(CMP.AlgorithmSuiteId.DBE(input.algorithmSuiteId.value))
+    if |fields| == 0 then
+      []
+    else if legend[0] == Header.ENCRYPT_AND_SIGN_LEGEND then
+      [fields[0]] + FilterEncrypted(fields[1..], legend[1..])
+    else
+      FilterEncrypted(fields[1..], legend[1..])
+  }
+
+  // Fail unless the field exists, and is a binary terminal
+  function method NeedBinary(data : StructuredDataMap, field : string): (result: Outcome<Error>)
+  {
+    if field !in data then
+      Fail(E("The field name " + field + " is required."))
+    else if !data[field].content.Terminal? then
+      Fail(E(field + " must be a Terminal."))
+    else if data[field].content.Terminal.typeId != BYTES_TYPE_ID then
+      Fail(E(field + " must be a binary Terminal."))
+    else
+      Pass
+  }
+
+  // Given a StructuredDataTerminal, return the canonical value for the type, for use in the footer checksum calculations
+  function method GetCanonicalType(value : StructuredDataTerminal, isEncrypted : bool)
+    : Result<Bytes, Error>
+  {
+    if isEncrypted then
+      :- Need(2 <= |value.value| < UINT64_LIMIT, E("Bad length."));
+      Success(UInt64ToSeq((|value.value| - 2) as uint64) + EncodeAscii("ENCRYPTED"))
+    else
+      :- Need(|value.value| < UINT64_LIMIT, E("Bad length."));
+      Success(UInt64ToSeq((|value.value|) as uint64) + EncodeAscii("PLAINTEXT") + value.typeId)
+  }
+
+  // Given a key value pair, return the canonical value for use in the footer checksum calculations
+  function method GetCanonicalItem(fieldName : CanonicalPath, value : StructuredData, isEncrypted : bool)
+    : Result<Bytes, Error>
+    requires value.content.Terminal?
+  {
+    var middle :- GetCanonicalType(value.content.Terminal, isEncrypted);
+    Success(fieldName + middle + GetValue(value))
+  }
+
+  // return the canonical representation of the StructuredData
+  // TODO - implement for real, once we have a spec; but this should still mostly fail at the right times.
+  // when looking for the data for a particular key, check encData first
+  // if it's not there, fall back to allData
+  function method CanonContent (
+    fields : seq<CanonicalPath>,      // remaining fields to be canonized
+    encFields : seq<CanonicalPath>,   // fields that are encrypted
+    encData : StructuredDataCanon,
+    allData : StructuredDataCanon,
+    canonized : Bytes := []   // output
+  ) : Result<Bytes, Error>
+    requires forall k <- fields :: k in allData
+    requires forall k <- encFields :: k in allData
+    requires forall k <- encData :: encData[k].content.Terminal?
+    requires forall k <- allData :: allData[k].content.Terminal?
+  {
+    if |fields| == 0 then
+      Success(canonized)
+    else
+      var data := if fields[0] in encData then encData[fields[0]] else allData[fields[0]];
+      var newPart :- GetCanonicalItem(fields[0], data, fields[0] in encFields);
+      CanonContent(fields[1..], encFields, encData, allData, canonized + newPart)
+  }
+
+  // Return the sum of the sizes of the given fields
+  function method SumValueSize(fields : seq<CanonicalPath>, data : StructuredDataCanon)
+    : nat
+    requires forall k <- fields :: k in data
+    requires forall k <- data :: data[k].content.Terminal?
+  {
+    if |fields| == 0 then
+      0
+    else
+      |data[fields[0]].content.Terminal.value| + SumValueSize(fields[1..], data)
+  }
+
+  // return the footer value for the StructuredData
+  // TODO - signatures et al
+  method GetFooter(
+    client: Primitives.AtomicPrimitivesClient,
+    key : Key,
+    edks : CMP.EncryptedDataKeyList,
+    alg : CMP.AlgorithmSuiteInfo,
+    signedFields : seq<CanonicalPath>,
+    encFields : seq<CanonicalPath>,
+    encData : StructuredDataCanon,
+    allData : StructuredDataCanon,
+    header : Bytes)
+    returns (ret : Result<Bytes, Error>)
+    requires ValidSuite(alg)
+    requires forall k <- signedFields :: k in allData
+    requires forall k <- encFields :: k in allData
+    requires forall k <- encData :: encData[k].content.Terminal?
+    requires forall k <- allData :: allData[k].content.Terminal?
+  {
+    var canon :- CanonContent(signedFields, encFields, encData, allData);
+    var data := header /* + AAD */ + canon; // TODO - is there an AAD?
+    var resultR := Digest.Digest(Prim.DigestInput(digestAlgorithm := Prim.SHA_384, message := data));
+    var canonicalHash :- resultR.MapFailure(e => AwsCryptographyPrimitives(e));
+    var result : Bytes := [];
+    for i := 0 to |edks| {
+      var input := Prim.HMacInput (
+        digestAlgorithm := alg.symmetricSignature.HMAC,
+        key := key, // TODO - mat.symmetricSigningKeys[i]
+        message := canonicalHash
+      );
+      var hashR := client.HMac(input);
+      var hash :- hashR.MapFailure(e => AwsCryptographyPrimitives(e));
+      :- Need(|hash| == 48, E("Bad hash length"));
+      result := result + hash;
+    }
+    if alg.signature.ECDSA? {
+      // TODO - once newer private-dafny is merged
+      // and also signatures are implemented
+      // then calculate real sig
+      result := result + canonicalHash + canonicalHash; // 96 bytes
+    }
+    return Success(result);
+  }
+
+  // return the appropriate EncryptionMaterials
+  method {:opaque} GetStructuredEncryptionMaterials(
+    cmm : CMP.ICryptographicMaterialsManager,
+    encryptionContext : Option<CMP.EncryptionContext>,
+    algorithmSuiteId: Option<CMP.DBEAlgorithmSuiteId>,
+    encryptedTerminalDataNum : nat,
+    totalEncryptedTerminalValuesSize : nat
+  )
+    returns (ret : Result<CMP.EncryptionMaterials, Error>)
+    ensures ret.Success? ==>
+      && var mat := ret.value;
+      && Materials.EncryptionMaterialsHasPlaintextDataKey(mat)
+      && ValidSuite(mat.algorithmSuite)
+
+      //= specification/structured-encryption/encrypt-structure.md#retrieve-encryption-materials
+      //= type=implication
+      //# This operation MUST obtain a set of encryption materials by calling
+      //# [Get Encryption Materials](https://github.com/awslabs/aws-encryption-sdk-specification/blob/master/framework/cmm-interface.md#get-encryption-materials)
+      //# on the input [CMM](#cmm).
+      && (|cmm.History.GetEncryptionMaterials| == |old(cmm.History.GetEncryptionMaterials)| + 1)
+      && Seq.Last(cmm.History.GetEncryptionMaterials).output.Success?
+      && var getEncIn := Seq.Last(cmm.History.GetEncryptionMaterials).input;
+      //= specification/structured-encryption/encrypt-structure.md#retrieve-encryption-materials
+      //= type=implication
+      //# - Encryption Context: If provided, this MUST be the [input encryption context](#encryption-context);
+      //# otherwise, this is an empty encryption context.
+      && (|| (encryptionContext.None? && getEncIn.encryptionContext == map[])
+          || (encryptionContext.Some? && getEncIn.encryptionContext == encryptionContext.value))
+
+      //= specification/structured-encryption/encrypt-structure.md#retrieve-encryption-materials
+      //= type=implication
+      //# - Commitment Policy: This MUST be
+      //# [REQUIRE_ENCRYPT_REQUIRE_DECRYPT](https://github.com/awslabs/aws-encryption-sdk-specification/blob/master/framework/commitment-policy.md#esdkrequire_encrypt_require_decrypt).
+      && getEncIn.commitmentPolicy == DBE_COMMITMENT_POLICY
+
+      //= specification/structured-encryption/encrypt-structure.md#retrieve-encryption-materials
+      //= type=implication
+      //# - Max Plaintext Length: This field MUST be the result of the calculation `encryptedTerminalDataNum * 2 + totalEncryptedTerminalValuesSize`
+      // - `encryptedTerminalDataNum` is the number of [Terminal Data](./structures.md#terminal-data)
+      //   in the [input Structured Data](#structured-data) being encrypted,
+      //   as defined by the [input Crypto Schema](#crypto-schema).
+      // - `totalEncryptedTerminalValuesSize` is the sum of the length of all [Terminal Values](./structures.md#terminal-value)
+      //   in the [input Structured Data](#structured-data) being encrypted,
+      //   as defined by the [input Crypto Schema](#crypto-schema).
+      && var maxLength :=  encryptedTerminalDataNum * 2 + totalEncryptedTerminalValuesSize;
+      && maxLength < INT64_MAX_LIMIT
+      && (getEncIn.maxPlaintextLength == Some(maxLength as int64))
+
+    modifies cmm.Modifies
+    requires cmm.ValidState()
+    ensures cmm.ValidState()
+  {
+    var maxLength :=  encryptedTerminalDataNum * 2 + totalEncryptedTerminalValuesSize;
+    :- Need(maxLength < INT64_MAX_LIMIT, E("Encrypted Size too long."));
+
+    var algorithmSuiteId := if algorithmSuiteId.Some? then
+      Some(CMP.AlgorithmSuiteId.DBE(algorithmSuiteId.value))
     else
       None;
 
-    var matR := input.cmm.GetEncryptionMaterials(
+    var matR := cmm.GetEncryptionMaterials(
       CMP.GetEncryptionMaterialsInput(
-        encryptionContext := input.encryptionContext.UnwrapOr(map[]),
+        encryptionContext := encryptionContext.UnwrapOr(map[]),
         commitmentPolicy := DBE_COMMITMENT_POLICY,
         algorithmSuiteId := algorithmSuiteId,
-        maxPlaintextLength := None
+        maxPlaintextLength := Some(maxLength as int64)
       )
     );
+
     var matOutput :- matR.MapFailure(e => AwsCryptographyMaterialProviders(e));
     var mat := matOutput.encryptionMaterials;
+    :- Need(Materials.EncryptionMaterialsHasPlaintextDataKey(mat), E("Encryption material has no key"));
+    var alg := mat.algorithmSuite;
+    :- Need(ValidSuite(alg), E("Invalid Algorithm Suite"));
+    var key : Key := mat.plaintextDataKey.value;
+    return Success(mat);
+  }
+
+  // for encryption, various canonized things
+  datatype EncryptCanon = EncryptCanon (
+    encFields_c : seq<CanonicalPath>,   // these fields should be encrypted
+    signedFields_c : seq<CanonicalPath>,// these fields should be signed, sorted
+    data_c : StructuredDataCanon        // all signed fields with canonized paths
+  )
+
+  // for decryption, data fields and schema, both plain field names and canonical path
+  datatype DecryptCanon = DecryptCanon (
+    signedFields_c : seq<CanonicalPath>,// these fields were signed, sorted
+    data_c : StructuredDataCanon        // all signed fields with canonized paths
+  )
+
+  // return the subset of "fields" which are ENCRYPT_AND_SIGN 
+  function method {:tailrecursion} FilterEncrypt(fields : seq<CanonicalPath>, fieldMap : CanonMap, schema : CryptoSchemaPlain)
+    : (ret : seq<CanonicalPath>)
+    requires forall k <- fields :: k in fieldMap
+    requires forall k <- fieldMap :: fieldMap[k] in schema
+    ensures forall k <- ret :: k in fields
+  {
+    if |fields| == 0 then
+      []
+    else
+      var act := schema[fieldMap[fields[0]]].content.Action;
+      if act == ENCRYPT_AND_SIGN then
+        [fields[0]] + FilterEncrypt(fields[1..], fieldMap, schema)
+      else
+        FilterEncrypt(fields[1..], fieldMap, schema)
+  }
+
+  // construct the EncryptCanon
+  function method {:opaque} CanonizeForEncrypt(tableName : GoodString, data : StructuredDataPlain, schema : CryptoSchemaPlain)
+    : (ret : Result<EncryptCanon, Error>)
+    requires schema.Keys == data.Keys
+    ensures ret.Success? ==>
+      && var r := ret.value;
+      && (forall k <- r.encFields_c :: k in r.data_c)
+      && (forall k <- r.signedFields_c :: k in r.data_c)
+      && (forall k <- r.encFields_c :: k in r.signedFields_c)
+  {
+    Paths.SimpleCanonUnique(tableName);
+    var fieldMap := map k <- data.Keys | schema[k].content.Action != DO_NOTHING :: Paths.SimpleCanon(tableName, k) := k;
+    var data_c := map k <- fieldMap :: k := data[fieldMap[k]];
+    var signedFields_c := Sets.ComputeSetToOrderedSequence2(data_c.Keys, ByteLess);
+    var encFields_c := FilterEncrypt(signedFields_c, fieldMap, schema);
+
+    Success(EncryptCanon(
+      encFields_c,
+      signedFields_c,
+      data_c
+    ))
+  }
+
+  // construct the DecryptCanon
+  function method {:opaque} CanonizeForDecrypt(tableName : GoodString, data : StructuredDataPlain, schema : AuthSchemaPlain)
+    : (ret : Result<DecryptCanon, Error>)
+    requires schema.Keys == data.Keys
+    ensures ret.Success? ==>
+      && var r := ret.value;
+      && (forall k <- r.signedFields_c :: k in r.data_c)
+  {
+    Paths.SimpleCanonUnique(tableName);
+    var fieldMap := map k <- data.Keys | schema[k].content.Action == SIGN :: Paths.SimpleCanon(tableName, k) := k;
+    var data_c := map k <- fieldMap :: k := data[fieldMap[k]];
+    var signedFields_c := Sets.ComputeSetToOrderedSequence2(data_c.Keys, ByteLess);
+
+    Success(DecryptCanon(
+      signedFields_c,
+      data_c
+    ))
+  }
+
+  method EncryptStructure(config: InternalConfig, input: EncryptStructureInput)
+    returns (output: Result<EncryptStructureOutput, Error>)
+    ensures output.Success? ==>
+      //= specification/structured-encryption/encrypt-structure.md#structured-data
+      //= type=implication
+      //# This Structured Data MUST be a [Structured Data Map](./structures.md#structured-data-map).
+      && input.plaintextStructure.content.DataMap?
+
+      //= specification/structured-encryption/encrypt-structure.md#structured-data
+      //= type=implication
+      //# This Structured Data MUST NOT already contain data located at the [header index](./header.md#header-index)
+      //# or the [footer index](./footer.md#footer-index).
+      && var plainRecord := input.plaintextStructure.content.DataMap;
+      && DataMapIsFlat(plainRecord)
+      && HeaderField !in plainRecord
+      && FooterField !in plainRecord
+
+      //= specification/structured-encryption/encrypt-structure.md#crypto-schema
+      //= type=implication
+      //# The Crypto Schema MUST explicitly configure a [Crypto Action](./structures.md#crypto-action) for every
+      //# [Terminal Data](./structures.md#terminal-data) that exists on the [input Structured Data](#structured-data),
+      //# and MUST NOT describe Crypto Actions for locations within the input Structured Data that either
+      //# do not exist, or contain non-Terminal Data structures;
+      //# otherwise, this operation operation MUST yield an error.
+      && input.cryptoSchema.content.SchemaMap?
+      && var cryptoSchema := input.cryptoSchema.content.SchemaMap;
+      && CryptoSchemaMapIsFlat(cryptoSchema)
+      && plainRecord.Keys == cryptoSchema.Keys
+  {
+    :- Need(input.plaintextStructure.content.DataMap?, E("Input structure must be a DataMap"));
+    :- Need(input.cryptoSchema.content.SchemaMap?, E("Input Crypto Schema must be a SchemaMap"));
+
+    var cryptoSchema := input.cryptoSchema.content.SchemaMap;
+    :- Need(CryptoSchemaMapIsFlat(cryptoSchema), E("Schema must be flat."));
+    :- Need(forall k <- cryptoSchema :: ValidString(k), E("Schema has bad field name."));
+
+    var plainRecord := input.plaintextStructure.content.DataMap;
+    :- Need(DataMapIsFlat(plainRecord), E("Input DataMap must be flat."));
+    :- Need(HeaderField !in plainRecord, E("The field name " + HeaderField + " is reserved."));
+    :- Need(FooterField !in plainRecord, E("The field name " + FooterField + " is reserved."));
+    :- Need(plainRecord.Keys == cryptoSchema.Keys, E("Schema must exactly match record"));
+
+    :- Need(ValidString(input.tableName), E("Bad Table Name"));
+    var canonData :- CanonizeForEncrypt(input.tableName, plainRecord, cryptoSchema);
+
+    var mat :- GetStructuredEncryptionMaterials(
+                input.cmm,
+                input.encryptionContext,
+                input.algorithmSuiteId,
+                |canonData.encFields_c|,
+                SumValueSize(canonData.encFields_c, canonData.data_c));
+
+    var key : Key := mat.plaintextDataKey.value;
+    var alg := mat.algorithmSuite;
 
     //= specification/structured-encryption/header.md#message-id
     //# Implementations MUST generate a fresh 256-bit random MessageID, from a cryptographically secure source, for each record encrypted.
-    var randBytes := Random.GenerateBytes(32);
+    var randBytes := Random.GenerateBytes(MSGID_LEN as int32);
     var msgID :- randBytes.MapFailure(e => Error.AwsCryptographyPrimitives(e));
-    var head :- Header.Create(input.tableName, input.cryptoSchema, msgID, mat.encryptionContext, mat.encryptedDataKeys);
+    var head :- Header.Create(input.tableName, input.cryptoSchema, msgID, mat);
 
-    // TODO: Currently implemented with "fake" encryption for ddb items.
-    // For each attribute that should be encrypted:
-    // - Concatenate typeId and value
-    // - Base64 encode
-    // - Concatenate THIS_IS_NOT_ENCRYPTED and output of the above
-    // - Create a new 'Terminal' with typeId 0x0001 (to be interpreted as string in DDB)
-    //   and value of the output of the above
-    :- Need(input.plaintextStructure.content.DataMap?
-        && input.cryptoSchema.content.SchemaMap?, StructuredEncryptionException(
-      message := "Unexpected Structured Data Item. Currently only implemented to accept DDB Items."
-    ));
-    
-    // Iterate through presumed DDB Item's attributes to perform "fake" encryption
-    var cryptoSchema := input.cryptoSchema.content.SchemaMap;
-    var ddbItem := input.plaintextStructure.content.DataMap;
-    var attributeValues := map[];
-    while cryptoSchema.Keys != {}
-    {
-      var attributeName :| attributeName in cryptoSchema;
-      :- Need(cryptoSchema[attributeName].content.Action?
-        && attributeName in ddbItem
-        && ddbItem[attributeName].content.Terminal?, StructuredEncryptionException(
-        message := "Unexpected Structured Data Item. Currently only implemented to accept DDB Items."
-      ));
-      if (cryptoSchema[attributeName].content.Action == CryptoAction.ENCRYPT_AND_SIGN) {
-        var attributeValue := ddbItem[attributeName].content.Terminal;
-        var concatValue := attributeValue.typeId + attributeValue.value;
-        var base64Value := Base64.Encode(concatValue);
-        var base64ValueAsBytes := UTF8.EncodeAscii(base64Value);
-        var finalValue := THIS_IS_NOT_ENCRYPTED + base64ValueAsBytes;
-        var transformedAttribute := StructuredData(
-          content := StructuredDataContent.Terminal(
-            Terminal := StructuredDataTerminal(
-              typeId := DDB_STRING_TYPE_ID,
-              value := finalValue
-            )
-          ),
-          attributes := None
-        );
-        attributeValues := attributeValues[attributeName:=transformedAttribute];
-      } else {
-        // passthrough
-        attributeValues := attributeValues[attributeName:=ddbItem[attributeName]];
-      }
+    var commitKey := Crypt.GetCommitKey(alg, key, head.msgID);
+    var headerSerialized :- Header.Serialize(config.primitives, alg, commitKey, head);
+    var headerAttribute := ValueToData(headerSerialized, BYTES_TYPE_ID);
 
-      cryptoSchema := cryptoSchema - {attributeName};
-    }
-    var headerSerialized :- Header.Serialize(config.primatives, head);
-    var headerString := Base64.Encode(headerSerialized);
-    var headerBytes := UTF8.EncodeAscii(headerString);
-    var headerAttribute := StructuredData(
-      content := StructuredDataContent.Terminal(
-        Terminal := StructuredDataTerminal(
-          typeId := BYTES_TYPE_ID,
-          value := headerBytes
-        )
-      ),
-      attributes := None
-    );
-    attributeValues := attributeValues["aws_ddb_head" := headerAttribute];
+    :- Need(|canonData.encFields_c| < (UINT32_LIMIT / 3), E("Too many encrypted fields"));
+    var encryptedItems :- Crypt.Encrypt(config.primitives, alg, key, head, canonData.encFields_c, canonData.data_c);
+
+    var result : map<string, StructuredData> := map k | k in plainRecord.Keys :: k :=
+      var c := Paths.SimpleCanon(input.tableName, k);
+      if c in encryptedItems then
+        encryptedItems[c]
+      else
+        plainRecord[k];
+
+    var footer :- GetFooter(config.primitives, key, mat.encryptedDataKeys, alg,
+                  canonData.signedFields_c, canonData.encFields_c, encryptedItems, canonData.data_c, headerSerialized);
+    var footerAttribute := ValueToData(footer, BYTES_TYPE_ID);
+
+    result := result + map[HeaderField := headerAttribute, FooterField := footerAttribute];
 
     var encryptOutput := EncryptStructureOutput(encryptedStructure := StructuredData(
       content := StructuredDataContent.DataMap(
-        DataMap := attributeValues
+        DataMap := result
       ),
       attributes := None
     ));
-    output := Success(encryptOutput);
+    return Success(encryptOutput);
   }
 
   predicate DecryptStructureEnsuresPublicly(
-    input: DecryptStructureInput, 
+    input: DecryptStructureInput,
     output: Result<DecryptStructureOutput, Error>) {
       // Input and output types must be the same, and this constraint is useful to Dafny users
     && (output.Success? && input.encryptedStructure.content.DataMap? ==> output.value.plaintextStructure.content.DataMap?)
     && (output.Success? && input.encryptedStructure.content.DataList? ==> output.value.plaintextStructure.content.DataList?)
     && (output.Success? && input.encryptedStructure.content.Terminal? ==> output.value.plaintextStructure.content.Terminal?)
   }
-  
-  function method E(message : string) : Error {
-    StructuredEncryptionException(message := message)
-  }
+
+  const ReservedAuthMap : AuthSchemaPlain := map[
+    HeaderField := DoNotSign, // The header field is authenticated in the footer via a separate mechanism
+    FooterField := DoNotSign
+  ]
 
   method DecryptStructure(config: InternalConfig, input: DecryptStructureInput)
-      returns (output: Result<DecryptStructureOutput, Error>)
+    returns (output: Result<DecryptStructureOutput, Error>)
+    ensures output.Success? ==>
+      && input.encryptedStructure.content.DataMap?
+      && var encRecord := input.encryptedStructure.content.DataMap;
+
+      //= specification/structured-encryption/header.md#header-index
+      //= type=implication
+      //# The header MUST exist at string index "aws_dbe_head" for
+      //# encrypted [Structured Data](./structures.md#structured-data).
+      && NeedBinary(encRecord, HeaderField).Pass?
+
+      //= specification/structured-encryption/footer.md#footer-index
+      //= type=implication
+      //# The header MUST exist at string index "aws_dbe_foot" for
+      //# encrypted [Structured Data](./structures.md#structured-data).
+      && NeedBinary(encRecord, FooterField).Pass?
   {
-    // TODO: Currently implemented with "fake" decryption for ddb itmes. This is currently brittle,
-    // but for now is useful to demonstrate that the attribute actions are being properly piped
-    // through the system.
-    :- Need(input.encryptedStructure.content.DataMap?, E("Unexpected Structured Data Item. Currently only implemented to accept DDB Items."));
-    
-    // Iterate through presumed DDB Item's attributes to perform "fake" encryption
-    var cryptoSchema := input.encryptedStructure.content.DataMap;
-    :- Need("aws_ddb_head" in cryptoSchema, E("aws_ddb_head field absent"));
-    var headerAttribute := cryptoSchema["aws_ddb_head"];
-    :- Need(headerAttribute.content.Terminal?, E("aws_ddb_head must be a Terminal"));
-    var headerBytes := headerAttribute.content.Terminal.value;
-    var headerStringR := UTF8.Decode(headerBytes);
-    var headerString :- headerStringR.MapFailure(e => E(e));
-    var headerSerializedR := Base64.Decode(headerString);
-    var headerSerialized :- headerSerializedR.MapFailure(e => E(e));
-    var head :- Header.Deserialize(config.primatives, headerSerialized);
+    :- Need(input.authenticateSchema.content.SchemaMap?, E("Authenticate Schema must be a SchemaMap"));
+    :- Need(AuthSchemaIsFlat(input.authenticateSchema.content.SchemaMap), E("Schema must be flat."));
+    :- Need(forall k <- input.authenticateSchema.content.SchemaMap :: ValidString(k), E("Schema has bad field name."));
+    var authSchema : AuthSchemaPlain := input.authenticateSchema.content.SchemaMap + ReservedAuthMap;
 
-    var attributeValues := map[];
-    while cryptoSchema.Keys != {}
-    {
-      var attributeName :| attributeName in cryptoSchema;
-      :- Need(cryptoSchema[attributeName].content.Terminal?, E("Unexpected Structured Data Item. Currently only implemented to accept DDB Items."));
-      var attributeValue := cryptoSchema[attributeName].content.Terminal;
-      // Since we are not storing the cryptoSchema that was used on encrypt,
-      // for our "fake" approach simply look for attributes that appear to be
-      // "fake" encrypted. Anyone testing integration with this fake encryption
-      // MUST NOT use the value "THIS_IS_NOT_ENCRYPTED" in their data set.
-      if (attributeValue.typeId == DDB_STRING_TYPE_ID
-          && |attributeValue.value| >= |THIS_IS_NOT_ENCRYPTED|
-          && attributeValue.value[..|THIS_IS_NOT_ENCRYPTED|] == THIS_IS_NOT_ENCRYPTED) {
-        // To "fake" decrypt:
-        // - String "THIS_IS_NOT_ENCRYPTED"
-        // - Base64 Decode the rest
-        // - Grab the first two bytes as typeId, the rest are the serialized value
-        var base64Value := attributeValue.value[|THIS_IS_NOT_ENCRYPTED|..];
-        var base64AsChar :- UTF8.Decode(base64Value)
-            .MapFailure(e => Types.StructuredEncryptionException( message := e ));
-        var concatValue :- Base64.Decode(base64AsChar)
-            .MapFailure(e => Types.StructuredEncryptionException( message := e ));
-        :- Need(|concatValue| >= 2, StructuredEncryptionException(
-          message := "Invalid 'fake' encryption: Missing typeId"
-        ));
-        var originalTypeId := concatValue[..2];
-        var originalValue := concatValue[2..];
-        var untransformedAttribute := StructuredData(
-          content := StructuredDataContent.Terminal(
-            Terminal := StructuredDataTerminal(
-              typeId := originalTypeId,
-              value := originalValue
-            )
-          ),
-          attributes := None
-        );
-        attributeValues := attributeValues[attributeName:=untransformedAttribute];
-      } else {
-        // else it is not "fake" encrypted, so pass through
-        attributeValues := attributeValues[attributeName:=cryptoSchema[attributeName]];
-      }
+    :- Need(input.encryptedStructure.content.DataMap?, E("Input structure must be a DataMap"));
+    :- Need(DataMapIsFlat(input.encryptedStructure.content.DataMap), E("Input DataMap must be flat."));
+    :- Need(authSchema.Keys == input.encryptedStructure.content.DataMap.Keys, E("Authenticate schema must match encrypted structure exactly."));
+    var encRecord : StructuredDataPlain := input.encryptedStructure.content.DataMap;
+    :- NeedBinary(encRecord, HeaderField);
+    :- NeedBinary(encRecord, FooterField);
 
-      cryptoSchema := cryptoSchema - {attributeName};
+    var headerSerialized := encRecord[HeaderField].content.Terminal.value;
+    var footerSerialized := encRecord[FooterField].content.Terminal.value;
+    var head :- Header.PartialDeserialize(headerSerialized);
+    var algorithmSuite :- head.GetAlgorithmSuite();
+
+    var matR := input.cmm.DecryptMaterials(
+      CMP.DecryptMaterialsInput (
+        algorithmSuiteId := algorithmSuite.id,
+        commitmentPolicy := DBE_COMMITMENT_POLICY,
+        encryptedDataKeys := head.dataKeys,
+        encryptionContext := head.encContext
+      )
+    );
+    var matOutput :- matR.MapFailure(e => AwsCryptographyMaterialProviders(e));
+    var mat := matOutput.decryptionMaterials;
+
+    :- Need(Materials.DecryptionMaterialsWithPlaintextDataKey(mat), E("Encryption material has no key"));
+    :- Need(ValidSuite(mat.algorithmSuite), E("Invalid Algorithm Suite"));
+    var alg := mat.algorithmSuite;
+    var key : Key := mat.plaintextDataKey.value;
+    var commitKey := Crypt.GetCommitKey(alg, key, head.msgID);
+    var ok :- head.verifyCommitment(config.primitives, alg, commitKey, headerSerialized);
+
+    :- Need(ValidString(input.tableName), E("Bad Table Name"));
+    var canonData :- CanonizeForDecrypt(input.tableName, encRecord, authSchema);
+
+    if |head.legend| < |canonData.signedFields_c| {
+      return Failure(E("Schema changed : something that was unsigned is now signed."));
     }
+    if |head.legend| > |canonData.signedFields_c| {
+      return Failure(E("Schema changed : something that was signed is now unsigned."));
+    }
+    assert |head.legend| == |canonData.signedFields_c|;
+
+    var encryptedFields := FilterEncrypted(canonData.signedFields_c, head.legend);
+    :- Need(|encryptedFields| < (UINT32_LIMIT / 3), E("Too many encrypted fields."));
+
+    var footer :- GetFooter(config.primitives, key, head.dataKeys, alg,
+                            canonData.signedFields_c, encryptedFields, map[], canonData.data_c, headerSerialized);
+    // TODO - footer checking is more complex than this
+    :- Need(footer == footerSerialized, E("Footer mismatch."));
+    var decryptedItems :- Crypt.Decrypt(config.primitives, alg, key, head, encryptedFields, canonData.data_c);
+
+    var result : map<string, StructuredData> := map k | k in encRecord.Keys :: k :=
+      var c := Paths.SimpleCanon(input.tableName, k);
+      if c in decryptedItems then
+        decryptedItems[c]
+      else
+        encRecord[k];
+
     var decryptOutput := DecryptStructureOutput(plaintextStructure := StructuredData(
       content := StructuredDataContent.DataMap(
-        DataMap := attributeValues
+        DataMap := result - {HeaderField, FooterField}
       ),
       attributes := None
     ));
+
     output := Success(decryptOutput);
   }
 }
