StructuredEncryption/src/Crypt.dfy
@@ -1,0 +1,240 @@
+// Copyright Amazon.com Inc. or its affiliates. All Rights Reserved.
+// SPDX-License-Identifier: Apache-2.0
+
+include "../Model/AwsCryptographyStructuredEncryptionTypes.dfy"
+include "../../private-aws-encryption-sdk-dafny-staging/AwsCryptographyPrimitives/src/AesKdfCtr.dfy"
+
+include "Header.dfy"
+include "Util.dfy"
+
+module StructuredEncryptionCrypt {
+  import opened Wrappers
+  import opened StandardLibrary
+  import opened StandardLibrary.UInt
+  import opened AwsCryptographyStructuredEncryptionTypes
+  import opened StructuredEncryptionUtil
+
+  import CMP = AwsCryptographyMaterialProvidersTypes
+  import Prim = AwsCryptographyPrimitivesTypes
+  import Aws.Cryptography.Primitives
+  import UTF8
+  import Header = StructuredEncryptionHeader
+  import HKDF
+  import AesKdfCtr
+
+
+  function method FieldKey(HKDFOutput : Bytes, offset : uint32)
+    : (ret : Result<Bytes, Error>)
+    requires |HKDFOutput| == KeySize
+    requires offset as nat * 3 < UINT32_LIMIT
+    ensures ret.Success? ==> |ret.value| == KeySize+NonceSize
+  {
+    Success((HKDFOutput+HKDFOutput)[..44]) // TODO - replace with below after next merge with private-dafny
+    //var keyR := AesKdfCtr.Stream(FieldKeyNonce(offset * 3), HKDFOutput, (KeySize+NonceSize) as uint32);
+    //keyR.MapFailure(e => AwsCryptographyPrimitives(e))
+  }
+
+  function method FieldKeyNonce(offset : uint32)
+    : (ret : Bytes)
+    ensures |ret| == 16 // NOT NonceSize
+    {
+      UTF8.EncodeAscii("AwsDbeField")
+      + [(KeySize+NonceSize) as uint8] // length
+      + UInt32ToSeq(offset)
+    }
+    
+  const LABEL_COMMITMENT_KEY := UTF8.EncodeAscii("AWS_DBE_COMMIT_KEY")
+  const LABEL_ENCRYPTION_KEY := UTF8.EncodeAscii("AWS_DBE_DERIVE_KEY")
+  
+  // suitable for header field
+  method GetCommitKey(alg : CMP.AlgorithmSuiteInfo, key : Key, msgID : MessageID)
+    returns (ret : Key)
+    requires ValidSuite(alg)
+  {
+    ret := HKDF.Hkdf(
+      alg.commitment.HKDF.hmac,
+      None, // salt
+      key, // ikm
+      LABEL_COMMITMENT_KEY + msgID, // info
+      alg.commitment.HKDF.outputKeyLength as int // length
+    );
+  }
+
+  datatype EncryptionSelector = DoEncrypt | DoDecrypt
+
+  // Encrypt a StructuredDataMap
+  method Encrypt(
+    client: Primitives.AtomicPrimitivesClient,
+    alg : CMP.AlgorithmSuiteInfo,
+    key : Key,
+    head : Header.PartialHeader,
+    fieldNames : seq<CanonicalPath>,
+    data : StructuredDataCanon)
+    returns (ret : Result<StructuredDataCanon, Error>)
+    requires forall k <- fieldNames :: k in data
+    requires |fieldNames| < (UINT32_LIMIT / 3)
+    requires ValidSuite(alg)
+
+    modifies client.Modifies
+    requires client.ValidState()
+    ensures client.ValidState()
+  {
+    ret := Crypt(DoEncrypt, client, alg, key, head, fieldNames, data);
+  }
+
+  // Decrypt a StructuredDataMap
+  method Decrypt(
+    client: Primitives.AtomicPrimitivesClient,
+    alg : CMP.AlgorithmSuiteInfo,
+    key : Key,
+    head : Header.PartialHeader,
+    fieldNames : seq<CanonicalPath>,
+    data : StructuredDataCanon)
+    returns (ret : Result<StructuredDataCanon, Error>)
+    requires forall k <- fieldNames :: k in data
+    requires |fieldNames| < (UINT32_LIMIT / 3)
+    requires ValidSuite(alg)
+
+    modifies client.Modifies
+    requires client.ValidState()
+    ensures client.ValidState()
+  {
+    ret := Crypt(DoDecrypt, client, alg, key, head, fieldNames, data);
+  }
+
+  // Encrypt or Decrypt a StructuredDataMap
+  // TODO - some guarantee that this encryption is being done in the right order
+  method Crypt(
+    mode : EncryptionSelector,
+    client: Primitives.AtomicPrimitivesClient,
+    alg : CMP.AlgorithmSuiteInfo,
+    key : Key,
+    head : Header.PartialHeader,
+    fieldNames : seq<CanonicalPath>,
+    data : StructuredDataCanon)
+    returns (ret : Result<StructuredDataCanon, Error>)
+    requires forall k <- fieldNames :: k in data
+    requires |fieldNames| < (UINT32_LIMIT / 3)
+    requires ValidSuite(alg)
+
+    modifies client.Modifies
+    requires client.ValidState()
+    ensures client.ValidState()
+  {
+    var fieldRootKey := HKDF.Hkdf(
+      alg.kdf.HKDF.hmac,
+      None, // salt
+      key, // ikm
+      LABEL_ENCRYPTION_KEY + head.msgID, // info
+      alg.kdf.HKDF.outputKeyLength as int // length
+    );
+    var result := CryptList(mode, client, alg, fieldRootKey, 0, fieldNames, data, map[]);
+    return result;
+  }
+
+  // Encrypt or Decrypt each entry in keys, putting results in output
+  method {:tailrecursion} CryptList(
+    mode : EncryptionSelector,
+    client: Primitives.AtomicPrimitivesClient,
+    alg : CMP.AlgorithmSuiteInfo,
+    fieldRootKey : Key,
+    offset : uint32,
+    fieldNames : seq<CanonicalPath>,
+    input : StructuredDataCanon,
+    output : StructuredDataCanon
+  )
+    returns (ret : Result<StructuredDataCanon, Error>)
+    requires forall k <- fieldNames :: k in input
+    requires (|fieldNames| + offset as nat) * 3 < UINT32_LIMIT
+    decreases |fieldNames|
+
+    modifies client.Modifies
+    requires client.ValidState()
+    ensures client.ValidState()
+  {
+    if |fieldNames| == 0 {
+      return Success(output);
+    }
+    var data;
+    if mode == DoEncrypt {
+      data :- EncryptTermina(client, alg, fieldRootKey, offset, fieldNames[0], input[fieldNames[0]].content.Terminal);
+    } else {
+      data :- DecryptTerminal(client, alg, fieldRootKey, offset, fieldNames[0], input[fieldNames[0]].content.Terminal);
+    }
+    var result := CryptList(mode, client, alg, fieldRootKey, offset+1, fieldNames[1..], input, output[fieldNames[0] := data]);
+    return result;
+  }
+
+  // Encrypt a single Terminal
+  method EncryptTermina(
+    client: Primitives.AtomicPrimitivesClient,
+    alg : CMP.AlgorithmSuiteInfo,
+    fieldRootKey : Key,
+    offset : uint32,
+    path : CanonicalPath,
+    data : StructuredDataTerminal
+  )
+    returns (ret : Result<StructuredData, Error>)
+    requires offset as nat * 3 < UINT32_LIMIT
+    ensures ret.Success? ==> ret.value.content.Terminal?
+
+    modifies client.Modifies
+    requires client.ValidState()
+    ensures client.ValidState()
+  {
+    var dataKey :- FieldKey(fieldRootKey, offset);
+    var encryptionKey : Key := dataKey[0..KeySize];
+    var nonce : Nonce := dataKey[KeySize..];
+    var value := data.value;
+
+    var encInput := Prim.AESEncryptInput(
+      encAlg := alg.encrypt.AES_GCM,
+      iv := nonce,
+      key := encryptionKey,
+      msg := value,
+      aad := path
+    );
+
+    var encOutR := client.AESEncrypt(encInput);
+    var encOut :- encOutR.MapFailure(e => AwsCryptographyPrimitives(e));
+    :- Need (|encOut.authTag| == AuthTagSize, E("Auth Tag Wrong Size."));
+    return Success(ValueToData(data.typeId + encOut.cipherText + encOut.authTag, BYTES_TYPE_ID));
+  }
+
+  // Decrypt a single Terminal
+  method DecryptTerminal(
+    client: Primitives.AtomicPrimitivesClient,
+    alg : CMP.AlgorithmSuiteInfo,
+    fieldRootKey : Key,
+    offset : uint32,
+    path : CanonicalPath,
+    data : StructuredDataTerminal
+  )
+    returns (ret : Result<StructuredData, Error>)
+    requires offset as nat * 3 < UINT32_LIMIT
+    ensures ret.Success? ==> ret.value.content.Terminal?
+
+    modifies client.Modifies
+    requires client.ValidState()
+    ensures client.ValidState()
+  {
+    var dataKey :- FieldKey(fieldRootKey, offset);
+    var encryptionKey : Key := dataKey[0..KeySize];
+    var nonce : Nonce := dataKey[KeySize..];
+    var value := data.value;
+
+    :- Need((AuthTagSize+2) <= |value|, E("cipherTxt too short."));
+    var decInput := Prim.AESDecryptInput(
+      encAlg := alg.encrypt.AES_GCM,
+      iv := nonce,
+      key := encryptionKey,
+      cipherTxt := value[TYPEID_LEN..|value| - AuthTagSize],
+      aad := path,
+      authTag := value[|value|-AuthTagSize..]
+    );
+
+    var decOutR := client.AESDecrypt(decInput);
+    var decOut :- decOutR.MapFailure(e => AwsCryptographyPrimitives(e));
+    return Success(ValueToData(decOut, value[..TYPEID_LEN]));
+  }
+}
