StructuredEncryption/test/TestFixtures.dfy
@@ -9,16 +9,13 @@ module TestFixtures {
   import opened StandardLibrary
   import opened UInt = StandardLibrary.UInt
   import opened AwsCryptographyStructuredEncryptionTypes
+  import opened StructuredEncryptionUtil
   import MaterialProviders
   import AwsCryptographyMaterialProvidersTypes
 
   const TEST_TYPE_ID : seq<uint8> := [0xFF, 0xFF];
-  const ENCRYPTED_TYPE_ID : seq<uint8> := [0x00, 0x01];
   const TEST_BLOB_VALUE : seq<uint8> := [0x21, 0x64, 0x6c, 0x72, 0x6f, 0x77, 0x20, 0x2c, 0x6f, 0x6c, 0x6c, 0x65, 0x68];
-  // The below is Con("THIS_IS_NOT_ENCRYPTED", Base64Encode(Con(TEST_TYPE_ID, TEST_BLOB_VALUE)))
-  const TEST_FAKE_ENCRYPTED_BLOB : seq<uint8> := [0x54, 0x48, 0x49, 0x53, 0x5f, 0x49, 0x53, 0x5f, 0x4e, 0x4f, 0x54, 0x5f,
-      0x45, 0x4e, 0x43, 0x52, 0x59, 0x50, 0x54, 0x45, 0x44, 0x2f, 0x2f, 0x38, 0x68, 0x5a, 0x47, 0x78, 0x79, 0x62, 0x33,
-      0x63, 0x67, 0x4c, 0x47, 0x39, 0x73, 0x62, 0x47, 0x56, 0x6f];
+
   const TEST_STRUCTURED_DATA := StructuredData(
     content := StructuredDataContent.DataMap(
       DataMap := map[
@@ -53,40 +50,7 @@ module TestFixtures {
     ),
     attributes := None()
   );
-  const TEST_STRUCTURED_DATA_ENCRYPTED := StructuredData(
-    content := StructuredDataContent.DataMap(
-      DataMap := map[
-        "foo" := StructuredData(
-          content := StructuredDataContent.Terminal(
-              Terminal := StructuredDataTerminal(
-                  value := TEST_FAKE_ENCRYPTED_BLOB,
-                  typeId := ENCRYPTED_TYPE_ID
-              )
-          ),
-          attributes := None()
-        ),
-        "bar" := StructuredData(
-          content := StructuredDataContent.Terminal(
-              Terminal := StructuredDataTerminal(
-                  value := TEST_BLOB_VALUE,
-                  typeId := TEST_TYPE_ID
-              )
-          ),
-          attributes := None()
-        ),
-        "fizzbuzz" := StructuredData(
-          content := StructuredDataContent.Terminal(
-              Terminal := StructuredDataTerminal(
-                  value := TEST_BLOB_VALUE,
-                  typeId := TEST_TYPE_ID
-              )
-          ),
-          attributes := None()
-        )
-      ]
-    ),
-    attributes := None()
-  );
+
   const TEST_CRYPTO_SCHEMA := CryptoSchema(
     content := CryptoSchemaContent.SchemaMap(
       SchemaMap := map[
